James C - down to one error in progress

isabelle/Chapter13_4_Evaluation.thy
@@ -33,49 +33,49 @@ lemma [simp]: "extract_constraint (PInR p) (Sum t1 t2) c ==>
       EX c'. extract_constraint p t2 c' & c = CInR t1 t2 c'"
 by (induction "PInR p" "Sum t1 t2" c rule: extract_constraint.induct, simp)
 
-inductive all_matches_complete :: "expr => type => bool"
+inductive all_matches_complete :: "expr => bool"
       and extract_constraints :: "rule list => type => constr => bool"
       and extract_constraint_rule :: "rule => type => constr => bool"
-where [simp]: "all_matches_complete (Var v) t" 
-    | [simp]: "all_matches_complete Zero Nat"
-    | [simp]: "all_matches_complete e Nat ==> all_matches_complete (Succ e) Nat"
-    | [simp]: "all_matches_complete e1 t ==> all_matches_complete e2 t ==> all_matches_complete e3 Nat ==> all_matches_complete (IsZ e1 e2 e3) t"
-    | [simp]: "all_matches_complete e (Arr t' t) ==> all_matches_complete (Lam t' e) t"
-    | [simp]: "all_matches_complete e1 (Arr t' t) ==> all_matches_complete e2 t' ==> all_matches_complete (Ap e1 e2) t" (* t' *)
-    | [simp]: "all_matches_complete e t ==> all_matches_complete (Fix t e) t"
-    | [simp]: "all_matches_complete Triv Unit"
-    | [simp]: "all_matches_complete e1 t1 ==> all_matches_complete e2 t2 ==> all_matches_complete (Pair e1 e2) (Prod t1 t2)"
-    | [simp]: "all_matches_complete e (Prod t1 t2) ==> all_matches_complete (ProjL e) t1" (* t2 *)
-    | [simp]: "all_matches_complete e (Prod t1 t2) ==> all_matches_complete (ProjR e) t2" (* t1 *)
-    | [simp]: "all_matches_complete e Void ==> all_matches_complete (Abort t e) t"
-    | [simp]: "all_matches_complete e t1 ==> all_matches_complete (InL t1 t2 e) (Sum t1 t2)"
-    | [simp]: "all_matches_complete e t2 ==> all_matches_complete (InR t1 t2 e) (Sum t1 t2)"
-    | [simp]: "all_matches_complete e t' ==> extract_constraints rs t' c ==> totally_satisfied t' c ==> all_matches_complete (Match e rs) t" (* t' *)
+where [simp]: "all_matches_complete (Var v)" 
+    | [simp]: "all_matches_complete Zero"
+    | [simp]: "all_matches_complete e ==> all_matches_complete (Succ e)"
+    | [simp]: "all_matches_complete e1 ==> all_matches_complete e2 ==> all_matches_complete e3 ==> all_matches_complete (IsZ e1 e2 e3)"
+    | [simp]: "all_matches_complete e ==> all_matches_complete (Lam t' e)"
+    | [simp]: "all_matches_complete e1 ==> all_matches_complete e2 ==> all_matches_complete (Ap e1 e2)"
+    | [simp]: "all_matches_complete e ==> all_matches_complete (Fix t e)"
+    | [simp]: "all_matches_complete Triv"
+    | [simp]: "all_matches_complete e1 ==> all_matches_complete e2 ==> all_matches_complete (Pair e1 e2)"
+    | [simp]: "all_matches_complete e ==> all_matches_complete (ProjL e)"
+    | [simp]: "all_matches_complete e ==> all_matches_complete (ProjR e)"
+    | [simp]: "all_matches_complete e ==> all_matches_complete (Abort t e)"
+    | [simp]: "all_matches_complete e ==> all_matches_complete (InL t1 t2 e)"
+    | [simp]: "all_matches_complete e ==> all_matches_complete (InR t1 t2 e)"
+    | [simp]: "all_matches_complete e ==> extract_constraints rs t c ==> totally_satisfied t c ==> all_matches_complete (Match e t rs)"
     | [simp]: "extract_constraints [] t Nothing"
     | [simp]: "extract_constraint_rule r t c1 ==> extract_constraints rs t c2 ==> extract_constraints (r # rs) t (Or c1 c2)"
-    | [simp]: "extract_constraint p t c ==> all_matches_complete e t ==> extract_constraint_rule (Rule p e) t c"
+    | [simp]: "extract_constraint p t c ==> all_matches_complete e ==> extract_constraint_rule (Rule p e) t c"
 
-inductive_cases [elim!]: "all_matches_complete (Var x) t"
-inductive_cases [elim!]: "all_matches_complete Zero t"
-inductive_cases [elim!]: "all_matches_complete (Succ x) t"
-inductive_cases [elim!]: "all_matches_complete (IsZ x y z) t"
-inductive_cases [elim!]: "all_matches_complete (Lam x y) t"
-inductive_cases [elim!]: "all_matches_complete (Ap x y) t"
-inductive_cases [elim!]: "all_matches_complete (Fix x y) t"
-inductive_cases [elim!]: "all_matches_complete Triv t"
-inductive_cases [elim!]: "all_matches_complete (Pair x y) t"
-inductive_cases [elim!]: "all_matches_complete (ProjL v) t"
-inductive_cases [elim!]: "all_matches_complete (ProjR v) t"
-inductive_cases [elim!]: "all_matches_complete (Abort x y) t"
-inductive_cases [elim!]: "all_matches_complete (InL x y z) t"
-inductive_cases [elim!]: "all_matches_complete (InR x y z) t"
-inductive_cases [elim!]: "all_matches_complete (Match x y) t"
+inductive_cases [elim!]: "all_matches_complete (Var x)"
+inductive_cases [elim!]: "all_matches_complete Zero"
+inductive_cases [elim!]: "all_matches_complete (Succ x)"
+inductive_cases [elim!]: "all_matches_complete (IsZ x y z)"
+inductive_cases [elim!]: "all_matches_complete (Lam x y)"
+inductive_cases [elim!]: "all_matches_complete (Ap x y)"
+inductive_cases [elim!]: "all_matches_complete (Fix x y)"
+inductive_cases [elim!]: "all_matches_complete Triv"
+inductive_cases [elim!]: "all_matches_complete (Pair x y)"
+inductive_cases [elim!]: "all_matches_complete (ProjL v)"
+inductive_cases [elim!]: "all_matches_complete (ProjR v)"
+inductive_cases [elim!]: "all_matches_complete (Abort x y)"
+inductive_cases [elim!]: "all_matches_complete (InL x y z)"
+inductive_cases [elim!]: "all_matches_complete (InR x y z)"
+inductive_cases [elim!]: "all_matches_complete (Match x y z)"
 inductive_cases [elim!]: "extract_constraints [] t c"
 inductive_cases [elim!]: "extract_constraints (x # y) t c"
 inductive_cases [elim!]: "extract_constraint_rule (Rule x y) t c"
 
 lemma [simp]: "types_from_pat p t ts ==> extract_constraint p t c ==> satisfies e c ==> EX s. matches s p e"
-proof (induction p t ts arbitrary: e rule: types_from_pat.induct)
+proof (induction p t ts arbitrary: e c rule: types_from_pat.induct)
 case tpwld
   have "matches [] Wild e" by simp
   thus ?case by (rule exI)
@@ -94,17 +94,56 @@ next case (tppar p1 t1 _ p2 t2 _)
   proof auto
     fix e1 e2 c1 c2
     assume "extract_constraint p1 t1 c1"
-       and "extract_constraint p2 t2 c2"
-       and "!!ee. extract_constraint p1 t1 (CPair c1 c2) \<Longrightarrow> satisfies ee (CPair c1 c2) \<Longrightarrow> \<exists>s. matches s p1 ee"
-       and "!!ee. extract_constraint p2 t2 (CPair c1 c2) \<Longrightarrow> satisfies ee (CPair c1 c2) \<Longrightarrow> \<exists>s. matches s p2 ee"
+       and "!!cc ee. extract_constraint p1 t1 cc \<Longrightarrow> satisfies ee cc \<Longrightarrow> \<exists>s. matches s p1 ee"
        and "satisfies e1 c1" 
-       and "satisfies e2 c2"
-    show "EX s. matches s (PPair p1 p2) (Pair e1 e2)" by simp sorry
+       and X: "extract_constraint p2 t2 c2"
+       and Y: "!!cc ee. extract_constraint p2 t2 cc \<Longrightarrow> satisfies ee cc \<Longrightarrow> \<exists>s. matches s p2 ee"
+       and Z: "satisfies e2 c2"
+    hence "EX s. matches s p1 e1" by simp
+    moreover from X Y Z have "EX s. matches s p2 e2" by simp
+    ultimately show "EX s. matches s (PPair p1 p2) (Pair e1 e2)"
+    proof auto
+      fix s1 s2
+      assume "matches s1 p1 e1" 
+         and "matches s2 p2 e2"
+      hence "matches (s1 @ s2) (PPair p1 p2) (Pair e1 e2)" by simp
+      thus "EX s. matches s (PPair p1 p2) (Pair e1 e2)" by (rule exI)
+    qed
   qed
 next case (tpinl p t1 _ t2)
-  thus ?case by simp sorry
+  hence "EX c'. extract_constraint p t1 c' & c = CInL t1 t2 c'" by auto
+  with tpinl show ?case
+  proof auto
+    fix e' c'
+    assume "extract_constraint p t1 c'"
+       and "!!cc ee. extract_constraint p t1 cc \<Longrightarrow> satisfies ee cc \<Longrightarrow> \<exists>s. matches s p ee"
+       and "satisfies e' c'" 
+    hence "EX s. matches s p e'" by simp
+    thus "EX s. matches s (PInL p) (InL t1 t2 e')"
+    proof auto
+      fix s
+      assume "matches s p e'" 
+      hence "matches s (PInL p) (InL t1 t2 e')" by simp
+      thus "EX s. matches s (PInL p) (InL t1 t2 e')" by (rule exI)
+    qed
+  qed
 next case (tpinr p t2 _ t1)
-  thus ?case by simp sorry
+  hence "EX c'. extract_constraint p t2 c' & c = CInR t1 t2 c'" by auto
+  with tpinr show ?case
+  proof auto
+    fix e' c'
+    assume "extract_constraint p t2 c'"
+       and "!!cc ee. extract_constraint p t2 cc \<Longrightarrow> satisfies ee cc \<Longrightarrow> \<exists>s. matches s p ee"
+       and "satisfies e' c'" 
+    hence "EX s. matches s p e'" by simp
+    thus "EX s. matches s (PInR p) (InR t1 t2 e')"
+    proof auto
+      fix s
+      assume "matches s p e'" 
+      hence "matches s (PInR p) (InR t1 t2 e')" by simp
+      thus "EX s. matches s (PInR p) (InR t1 t2 e')" by (rule exI)
+    qed
+  qed
 qed
 
 inductive eval :: "expr => expr => bool"
@@ -125,9 +164,9 @@ where esuc [simp]: "eval n n' ==> eval (Succ n) (Succ n')"
     | eabt [simp]: "eval e e' ==> eval (Abort t e) (Abort t e')"
     | einl [simp]: "eval e e' ==> eval (InL t t' e) (InL t t' e')"
     | einr [simp]: "eval e e' ==> eval (InR t t' e) (InR t t' e')"
-    | emt1 [simp]: "eval e e' ==> eval (Match e rs) (Match e' rs)"
-    | emt2 [simp]: "is_val e ==> matches s p e ==> eval (Match e (Rule p e2 # rs)) (apply_subst s e2)"
-    | emt3 [simp]: "is_val e ==> no_match e p ==> eval (Match e rs) e' ==> eval (Match e (Rule p e2 # rs)) e'"
+    | emt1 [simp]: "eval e e' ==> eval (Match e t rs) (Match e' t rs)"
+    | emt2 [simp]: "is_val e ==> matches s p e ==> eval (Match e t (Rule p e2 # rs)) (apply_subst s e2)"
+    | emt3 [simp]: "is_val e ==> no_match e p ==> eval (Match e t rs) e' ==> eval (Match e t (Rule p e2 # rs)) e'"
 
 theorem preservation: "eval e e' ==> typecheck env e t ==> typecheck env e' t"
 proof (induction e e' arbitrary: t env rule: eval.induct)
@@ -170,24 +209,18 @@ next case einl
   thus ?case by auto
 next case einr
   thus ?case by auto
-next case (emt1 e e' rs)
-  hence "EX t1. typecheck env e t1 & typecheck_rules env rs t1 t" by auto
+next case (emt1 e e' t1 rs)
+  hence "typecheck env e t1 & typecheck_rules env rs t1 t" by auto
+  moreover with emt1 have "typecheck env e' t1" by simp
+  ultimately show ?case by simp
+next case (emt2 e s p t1 e' rs)
   thus ?case
   proof auto
-    fix t1 c
-    assume "typecheck env e t1"
-       and "typecheck_rules env rs t1 t"
-    moreover with emt1 have "typecheck env e' t1" by simp
-    ultimately show "typecheck env (Match e' rs) t" by simp
-  qed
-next case (emt2 e s p e' rs)
-  thus ?case
-  proof auto
-    fix t1 ts
+    fix ts
     assume W: "is_val e" 
        and V: "matches s p e" 
        and Z: "typecheck env e t1" 
-       and Y: "types_from_pat p t1 ts" 
+       and Y: "types_from_pat p t1 ts"
        and X: "typecheck (extend_env ts env) e' t" 
     have "types_from_pat p t1 ts ==> typecheck env e t1 ==> is_val e ==> (EX s. typecheck_subst env s ts & matches s p e) | no_match e p" by simp
     with Y Z W V have "EX s. typecheck_subst env s ts & matches s p e" by simp
@@ -201,11 +234,11 @@ next case (emt2 e s p e' rs)
     qed
     with X show "typecheck env (apply_subst s e') t" by simp
   qed
-next case (emt3 e p rs e' e2)
+next case emt3
   thus ?case by auto
 qed
 
-theorem progress: "typecheck env e t ==> env = empty_map ==> all_matches_complete e t ==> is_val e | (EX e'. eval e e')"
+theorem progress: "typecheck env e t ==> env = empty_map ==> all_matches_complete e ==> is_val e | (EX e'. eval e e')"
     and "typecheck_rules env rs t1 t ==> env = empty_map ==> True"
     and "typecheck_rule env r t1 t ==> env = empty_map ==> True"
 proof (induction env e t rule: typecheck_typecheck_rules_typecheck_rule.inducts)
@@ -256,10 +289,7 @@ next case (trec env e e0 t e1)
 next case tlam
   thus ?case by simp
 next case (tapp env e1 t2 t e2)
-  from tapp have "typecheck env e1 (Arr t2 t)" by simp
-  from tapp have "typecheck env e2 t2" by simp
-  from tapp have "is_val e2 \<or> (\<exists>a. eval e2 a)" by auto sorry
-  thus ?case
+  show ?case
   proof (cases "is_val e1")
   case True
     with tapp have "EX v. e1 = Lam t2 v & typecheck (extend_at env 0 t2) v t" by (simp add: canonical_arr)
@@ -275,7 +305,7 @@ next case (tapp env e1 t2 t e2)
         thus "EX x. eval (Ap (Lam t2 v) e2) x" by auto
       qed
     next case False
-      with tapp have "\<exists>a. eval e2 a" by auto sorry
+      with tapp have "\<exists>a. eval e2 a" by auto
       thus ?thesis
       proof auto
         fix a
@@ -286,7 +316,7 @@ next case (tapp env e1 t2 t e2)
       qed
     qed
   next case False
-    with tapp have "\<exists>a. eval e1 a" by auto sorry
+    with tapp have "\<exists>a. eval e1 a" by auto
     thus ?thesis
     proof auto
       fix a
@@ -346,7 +376,7 @@ next case (tprl env e t1 t2)
       thus "EX a. eval (ProjL (Pair e1 e2)) a" by auto
     qed
   next case False
-    with tprl have "EX a. eval e a" by auto sorry
+    with tprl have "EX a. eval e a" by auto
     thus ?thesis
     proof auto
       fix a
@@ -369,7 +399,7 @@ next case (tprr env e t1 t2)
       thus "EX a. eval (ProjR (Pair e1 e2)) a" by auto
     qed
   next case False
-    with tprr have "EX a. eval e a" by auto sorry
+    with tprr have "EX a. eval e a" by auto
     thus ?thesis
     proof auto
       fix a
@@ -409,17 +439,19 @@ next case (tmch env e t1 rs t2)
     hence "is_val e" by simp
     from tmch have "typecheck env e t1" by simp
     from tmch have "typecheck_rules env rs t1 t2" by simp
+    from tmch have "all_matches_complete e \<Longrightarrow> is_val e | (EX a. eval e a)" by simp
+    from tmch have "all_matches_complete (Match e t1 rs)" by simp
 
-    hence "EX a. eval (Match e rs) a" by auto sorry
+    hence "EX a. eval (Match e t1 rs) a" by auto sorry
     thus ?thesis by simp
   next case False
-    with tmch have "EX a. eval e a" by auto sorry
+    with tmch have "EX a. eval e a" by auto
     thus ?thesis
     proof auto
       fix a
       assume "eval e a"
-      hence "eval (Match e rs) (Match a rs)" by simp
-      thus "EX x. eval (Match e rs) x" by auto
+      hence "eval (Match e t1 rs) (Match a t1 rs)" by simp
+      thus "EX x. eval (Match e t1 rs) x" by auto
     qed
   qed
 next case tnil
